bigodafny/solutions-verified/1011/1011_368.dfy
@@ -20,14 +20,30 @@
 include "../../prelude.dfy"
 import opened Prelude
 
-method Solve(n: int) returns (output: string)
+method Solve(n: int) returns (output: string, ghost steps: nat)
+  requires n >= 1
+  ensures steps <= 8 * n + 5
 {
+  steps := 1;
   var a := 1;
   var b := 1;
   while a * b < n
+    invariant a >= 1 && b >= 1
+    invariant steps <= 2 * (a * b) - 1
+    invariant a * b <= 2 * n + 1
     decreases n - a * b
   {
-    if a < b { a := a + 1; } else { b := b + 1; }
+    var oa, ob := a, b;
+    if a < b {
+      a := a + 1;
+    } else {
+      b := b + 1;
+    }
+    assert a * b == oa * ob + (if oa < ob then ob else oa);
+    assert (if oa < ob then ob else oa) <= oa * ob;
+    assert a * b <= 2 * (oa * ob);
+    steps := steps + 2;
   }
   output := IntToString(a + b);
+  steps := steps + 1;
 }
